iris/ProofVirtioDiskRwD.v
@@ -52,6 +52,7 @@ Require Import WpSmodeHalf.
 Require Import VirtioModel VirtioQueue DiskPtsto VirtioProto DiskInv.
 Require Import VirtioModel.
 Require Import WpUart.
+Require Import PermInv.
 Require Import CodeVirtioDiskRw.
 Require Import VirtioDiskRwDefs.
 Require Import Riscv.rv64d_types Riscv.rv64d Riscv.riscv_extras.
@@ -769,9 +770,13 @@ End VdrwdLeaves.
 (* ===================================================================== *)
 
 (* the slot [virtio_disk_rw] publishes *)
-Definition vdrwd_slot (b : Arch.pa) (h : nat) (wr sector : SailStdpp.Values.mword 64)
+(* [kq] is the crash-permit key ([VirtioQueue.vs_perm]); it comes FIRST so
+   that every downstream statement about the published slot threads it as a
+   leading parameter, exactly like a section variable would. *)
+Definition vdrwd_slot (kq : nat * positive) (b : Arch.pa) (h : nat)
+    (wr sector : SailStdpp.Values.mword 64)
     (bs : list (bv 8)) : vslot :=
-  rw_slot h (vdrw_ty wr) sector (b_data b) (d_info_status h) bs.
+  rw_slot h (vdrw_ty wr) sector (b_data b) (d_info_status h) bs kq.
 
 (* whether the request is a WRITE, as the pin sees it *)
 Definition vdrwd_out (wr : SailStdpp.Values.mword 64) : bool :=
@@ -846,7 +851,8 @@ Proof. vm_compute. reflexivity. Qed.
 
 (* THE pure half: a pin that CONTAINS the sixteen windows (and, for a write
    request, the payload) parses to exactly the request the driver meant. *)
-Lemma vdrwd_mk_pin (pd pav pu : SailStdpp.Values.mword 64) (b : Arch.pa)
+Lemma vdrwd_mk_pin (kq : nat * positive)
+    (pd pav pu : SailStdpp.Values.mword 64) (b : Arch.pa)
     (np h m2 t : nat) (wr sector : SailStdpp.Values.mword 64)
     (bs : list (bv 8)) (pin mbuf : _) :
   (h < 8)%nat -> (m2 < 8)%nat -> (t < 8)%nat ->
@@ -855,13 +861,13 @@ Lemma vdrwd_mk_pin (pd pav pu : SailStdpp.Values.mword 64) (b : Arch.pa)
   (bv_unsigned (vdrw_ty wr) = virtio_blk_t_out ->
      range_map (b_data b) 1024 (fun j => bs !!! j) ⊆ pin) ->
   d_info_status h ∉ pa_range (b_data b) 1024 ->
-  slot_pin_ok (virtio_init_cfg pd pav pu) np (vdrwd_slot b h wr sector bs) pin.
+  slot_pin_ok (virtio_init_cfg pd pav pu) np (vdrwd_slot kq b h wr sector bs) pin.
 Proof.
   intros Hh Hm Ht Hlen Hsub Hbuf Hstat.
   destruct (vdrwc_ty_flags wr) as [Htyv Hflags].
   unfold vdrwd_slot.
   apply (mk_pin_slot_ok (virtio_init_cfg pd pav pu) np pd pin h m2 t
-           (d_ops h) (b_data b) (d_info_status h) (vdrw_ty wr) sector bs).
+           (d_ops h) (b_data b) (d_info_status h) (vdrw_ty wr) sector bs kq).
   - reflexivity.
   - reflexivity.
   - exact Hh.
@@ -992,7 +998,8 @@ Section VdrwdPinBuild.
      caller's buffer become the pin and the writable footprint the publish
      accessor consumes -- plus, for a WRITE, the payload moves from the
      writable side into the pin. *)
-  Lemma vdrwd_pin_res (pd pav pu : SailStdpp.Values.mword 64) (b : Arch.pa)
+  Lemma vdrwd_pin_res (kq : nat * positive)
+      (pd pav pu : SailStdpp.Values.mword 64) (b : Arch.pa)
       (np h m2 t : nat) (wr sector : SailStdpp.Values.mword 64)
       (bs bsl : list (bv 8)) :
     (h < 8)%nat -> (m2 < 8)%nat -> (t < 8)%nat ->
@@ -1006,9 +1013,9 @@ Section VdrwdPinBuild.
     vdrw_chain pd b h m2 t wr sector -∗
     ([∗ list] j ↦ x ∈ bs, pa_add (b_data b) j ↦ₘ x) -∗
     ∃ pin wrb,
-      ⌜slot_pin_ok (virtio_init_cfg pd pav pu) np (vdrwd_slot b h wr sector bsl) pin⌝ ∗
-      ⌜dom wrb = slot_wr (vdrwd_slot b h wr sector bsl)⌝ ∗
-      ⌜slot_wr (vdrwd_slot b h wr sector bsl) ## dom pin⌝ ∗
+      ⌜slot_pin_ok (virtio_init_cfg pd pav pu) np (vdrwd_slot kq b h wr sector bsl) pin⌝ ∗
+      ⌜dom wrb = slot_wr (vdrwd_slot kq b h wr sector bsl)⌝ ∗
+      ⌜slot_wr (vdrwd_slot kq b h wr sector bsl) ## dom pin⌝ ∗
       (* THE STRUCTURE OF THE PIN, for P6: the residue after the interrupt
          handler splits the avail-ring entry back off is exactly the fifteen
          formatted windows (plus a write's payload), pairwise disjoint. *)
@@ -1132,7 +1139,7 @@ Section VdrwdPinBuild.
       iFrame "Hpin Hst Hib Hbd Hrm Hrt".
       destruct Hpmok as [Hdring Hpmok'].
       iPureIntro. split_and!.
-      + apply (vdrwd_mk_pin pd pav pu b np h m2 t wr sector bsl _
+      + apply (vdrwd_mk_pin kq pd pav pu b np h m2 t wr sector bsl _
                  (range_map (b_data b) 1024 (fun j => bs !!! j))
                  Hh Hm Ht Hlensl).
         * exact Hsub.
@@ -1172,7 +1179,7 @@ Section VdrwdPinBuild.
       iFrame "Hpin Hwrb Hib Hbd Hrm Hrt".
       destruct Hpmok as [Hdring Hpmok'].
       iPureIntro. split_and!.
-      + apply (vdrwd_mk_pin pd pav pu b np h m2 t wr sector bsl _ ∅
+      + apply (vdrwd_mk_pin kq pd pav pu b np h m2 t wr sector bsl _ ∅
                  Hh Hm Ht Hlensl).
         * exact Hsub.
         * intro Hc. exfalso. rewrite Hc Z.eqb_refl in Hout. discriminate.
@@ -1328,9 +1335,10 @@ Lemma vdrwd_dom_tr_ins {A : Type} (np : nat) (fl pk : gmap nat A)
 Proof. intro H. rewrite !dom_insert_L H. set_solver. Qed.
 
 (* the slot the publisher records really does describe the caller's buffer *)
-Lemma vdrwd_slot_link (b : Arch.pa) (h : nat) (wr sector : SailStdpp.Values.mword 64)
+Lemma vdrwd_slot_link (kq : nat * positive) (b : Arch.pa) (h : nat)
+    (wr sector : SailStdpp.Values.mword 64)
     (bs : list (bv 8)) :
-  (h < 8)%nat -> slot_buf_link (vdrwd_slot b h wr sector bs) b.
+  (h < 8)%nat -> slot_buf_link (vdrwd_slot kq b h wr sector bs) b.
 Proof.
   intro Hh. unfold slot_buf_link, vdrwd_slot.
   exists h. cbn [rw_slot vs_req vr_head vr_status vr_buf].
@@ -1342,18 +1350,20 @@ Proof.
   - unfold vs_len. cbn [rw_slot vs_req vr_len]. exact vdrwd_len1024.
 Qed.
 
-Lemma vdrwd_slot_head (b : Arch.pa) (h : nat) (wr sector : SailStdpp.Values.mword 64)
+Lemma vdrwd_slot_head (kq : nat * positive) (b : Arch.pa) (h : nat)
+    (wr sector : SailStdpp.Values.mword 64)
     (bs : list (bv 8)) :
-  (h < 8)%nat -> sl_head (vdrwd_slot b h wr sector bs) = h.
+  (h < 8)%nat -> sl_head (vdrwd_slot kq b h wr sector bs) = h.
 Proof.
   intro Hh. unfold sl_head, vdrwd_slot. cbn [rw_slot vs_req vr_head].
   rewrite (bv16_small h Hh). lia.
 Qed.
 
-Lemma vdrwd_slot_off (b : Arch.pa) (h : nat) (wr sector : SailStdpp.Values.mword 64)
+Lemma vdrwd_slot_off (kq : nat * positive) (b : Arch.pa) (h : nat)
+    (wr sector : SailStdpp.Values.mword 64)
     (bs : list (bv 8)) (o : Z) :
   bv_unsigned sector = o ->
-  vs_sector_off (vdrwd_slot b h wr sector bs) = (o * 512)%Z.
+  vs_sector_off (vdrwd_slot kq b h wr sector bs) = (o * 512)%Z.
 Proof.
   intro Ho. unfold vs_sector_off, vdrwd_slot, virtio_sector_size.
   cbn [rw_slot vs_req vr_sector]. rewrite Ho. reflexivity.
@@ -1385,7 +1395,8 @@ Section VdrwdP4.
 
   Local Ltac pcstep := apply bv_eq; vm_compute; reflexivity.
 
-  Lemma wp_vdrw_p4 (γu : uart_names) (γd : disk_names) (Φ : mval -> iProp Σ) (pme : Arch.pa)
+  Lemma wp_vdrw_p4 (kq : nat * positive)
+      (γu : uart_names) (γd : disk_names) (Φ : mval -> iProp Σ) (pme : Arch.pa)
       (M : regfile) (av : nat)
       (pd pav pu : SailStdpp.Values.mword 64) (b : Arch.pa)
       (wr sector : SailStdpp.Values.mword 64)
@@ -1407,6 +1418,11 @@ Section VdrwdP4.
     vdrw_chain pd b h m2 t wr sector -∗
     ([∗ list] j ↦ x ∈ bs_buf, pa_add (b_data b) j ↦ₘ x) -∗
     disk_bytes γd sec_off bs_disk -∗
+    (* THE CRASH PERMIT's token, deposited before the chain was formatted and
+       spent into the published slot here (PermInv.v).  It is the TIMELESS
+       skeleton of the client's view shift: the shift itself is in
+       [perm_inv], keyed by [kq], and the DMA completion runs it. *)
+    perm_pend (dn_perm γd) kq -∗
     ( ∀ (M1 : regfile) pin,
         ⌜(forall r : mword 5, is_cs_idx r = true -> M1 !!! Regidx r = M !!! Regidx r)
          /\ M1 !!! Regidx Ra1 = M !!! Regidx Ra1⌝ -∗
@@ -1419,11 +1435,11 @@ Section VdrwdP4.
         sie_cap_gpr M1 av false pme -∗
         pc_is (mword_of_int (VRW + 0x186) : mword 64) -∗
         vdrw_body γd pd pav (S np) nr
-                  (<[ np := DClaim b (vdrwd_slot b h wr sector
+                  (<[ np := DClaim b (vdrwd_slot kq b h wr sector
                                         (vdrwd_sldata wr bs_buf bs_disk))
                                    (h, m2, t) pin ]> fl) pk
                   (<[ np := (h, m2, t) ]> tr) fr -∗
-        disk_claim γd np (DClaim b (vdrwd_slot b h wr sector
+        disk_claim γd np (DClaim b (vdrwd_slot kq b h wr sector
                                       (vdrwd_sldata wr bs_buf bs_disk))
                                  (h, m2, t) pin) -∗
         vdrw_slot_rest m2 -∗ vdrw_slot_rest t -∗
@@ -1432,7 +1448,7 @@ Section VdrwdP4.
   Proof.
     intros Htok Hdisj0 Hfrh Hfrm Hfrt Hlenbuf Hlendisk Hbufkd Hoff Ha0 Ha5.
     destruct Htok as (Hhm & Hht & Hmt & Hh8 & Hm8 & Ht8). cbn in Hh8, Hm8, Ht8.
-    iIntros "Hcg #Htext Hpc #Hdinv #Hgeom Hbody Hchain Hbuf Hdisk Hcont".
+    iIntros "Hcg #Htext Hpc #Hdinv #Hgeom Hbody Hchain Hbuf Hdisk Hpend Hcont".
     iDestruct (sie_cap_gpr_kmap_claims with "Hcg") as "[#Hkm Hcg]".
     iDestruct (disk_geom_static with "Hgeom") as %(Hspd & Hspav & _).
     iPoseProof "Hgeom" as "Hgeom2".
@@ -1681,7 +1697,7 @@ Section VdrwdP4.
     { unfold vdrwd_sldata. destruct (vdrwd_out wr); assumption. }
     assert (Hbsl : vdrwd_out wr = true -> vdrwd_sldata wr bs_buf bs_disk = bs_buf).
     { unfold vdrwd_sldata. intro Ho. rewrite Ho. reflexivity. }
-    iDestruct (vdrwd_pin_res pd pav pu b np h m2 t wr sector bs_buf
+    iDestruct (vdrwd_pin_res kq pd pav pu b np h m2 t wr sector bs_buf
                  (vdrwd_sldata wr bs_buf bs_disk)
                  Hh8 Hm8 Ht8 Hlenbuf Hlensl Hbsl Hspd Hspav Hsbuf
                  with "Hkm Hcell Hchain Hbuf") as
@@ -1694,18 +1710,22 @@ Section VdrwdP4.
     iApply (wp_vdrwd_sh_publish γu γd pme Φ pd pav pu
               (mword_of_int (VRW + 0x17e) : mword 64) Ra5 Ra4
               (mword_of_int 2 : mword 12) N8 av np
-              (vdrwd_slot b h wr sector (vdrwd_sldata wr bs_buf bs_disk)) pin wrb
+              (vdrwd_slot kq b h wr sector (vdrwd_sldata wr bs_buf bs_disk)) pin wrb
               Hidxa3 HN8sv Hpinok Hwrbdom Hwrpin
-              with "Hcg Hpc Hi17e Hdinv Hgeom Hpub Hpin Hwrb [Hdisk] [-]").
+              with "Hcg Hpc Hi17e Hdinv Hgeom Hpub Hpin Hwrb [Hdisk Hpend] [-]").
     { iExists bs_disk. iSplitR.
       - iPureIntro. unfold vs_len, vdrwd_slot. cbn [rw_slot vs_req vr_len].
         rewrite vdrwd_len1024. exact Hlendisk.
       - iSplitR.
         + iPureIntro. unfold vs_is_out, vs_data, vdrwd_slot, vdrwd_sldata, vdrwd_out.
           cbn [rw_slot vs_req vr_type]. intro Ho. rewrite Ho. reflexivity.
-        + rewrite (vdrwd_slot_off b h wr sector (vdrwd_sldata wr bs_buf bs_disk)
-                     (bv_unsigned sector) eq_refl) Hoff.
-          iExact "Hdisk". }
+        + iSplitL "Hdisk".
+          * rewrite (vdrwd_slot_off kq b h wr sector
+                       (vdrwd_sldata wr bs_buf bs_disk)
+                       (bv_unsigned sector) eq_refl) Hoff.
+            iExact "Hdisk".
+          * (* [vs_perm (vdrwd_slot kq …) = kq] by conversion *)
+            iExact "Hpend". }
     iIntros "Hcg Hpc Hpub Hrcpt".
     assert (Hp182 : add_vec_int (mword_of_int (VRW + 0x17e) : mword 64) 4
                     = mword_of_int (VRW + 0x182)) by pcstep.
@@ -1720,7 +1740,7 @@ Section VdrwdP4.
                     = mword_of_int (VRW + 0x186)) by pcstep.
     iEval (rewrite Hp186) in "Hpc".
     (* ---- the claim, and the rebuilt lock resource ---- *)
-    set (V := DClaim b (vdrwd_slot b h wr sector (vdrwd_sldata wr bs_buf bs_disk))
+    set (V := DClaim b (vdrwd_slot kq b h wr sector (vdrwd_sldata wr bs_buf bs_disk))
                      (h, m2, t) pin).
     iMod (ghost_map_insert np V
             (vdrwd_fresh_pos np nr fl pk Hle Hdfl Hpkb)
@@ -1731,9 +1751,9 @@ Section VdrwdP4.
     { iSplitR "Hflm"; [| iExact "Hflm"]. rewrite /flight_res /V.
       cbn [dc_buf dc_slot dc_tri dc_pin].
       iSplitR; [iPureIntro;
-        exact (vdrwd_slot_link b h wr sector (vdrwd_sldata wr bs_buf bs_disk) Hh8)|].
+        exact (vdrwd_slot_link kq b h wr sector (vdrwd_sldata wr bs_buf bs_disk) Hh8)|].
       iFrame "Hrcpt Hbd".
-      rewrite (vdrwd_slot_head b h wr sector (vdrwd_sldata wr bs_buf bs_disk) Hh8).
+      rewrite (vdrwd_slot_head kq b h wr sector (vdrwd_sldata wr bs_buf bs_disk) Hh8).
       iExact "Hib". }
     iApply ("Hcont" $! N8 pin with "[%] [%] Hcg Hpc [-Hfrag Hrm Hrt] [Hfrag] Hrm Hrt").
     { split.
